wip Type-dependent functions

theories/L/Datatypes/LOptions.v
@@ -1,31 +1,64 @@
 From Undecidability.L Require Import Tactics.LTactics Datatypes.LBool Tactics.GenEncode.
 
 (** ** Encoding of option type *)
-Section Fix_X.
-  Variable X:Type.
-  Variable intX : registered X.
+(* Section Fix_X. *)
+(*   Variable X:Type. *)
+(*   Variable intX : registered X. *)
 
+(*   (*Run TemplateProgram (tmGenEncode "option_enc" (@option X)).*) 
+Hint Resolve option_enc_correct : Lrewrite.
 
-  Run TemplateProgram (tmGenEncode "option_enc" (option X)).
-  Hint Resolve option_enc_correct : Lrewrite.
+End Fix_X.*)
 
-  (* now we must register the non-constant constructors*)
-
-  Global Instance term_Some : computableTime' (@Some X) (fun _ _ => (1,tt)).
-  Proof.
-    extract constructor.
-    solverec.
-  Defined.
   
-  Lemma oenc_correct_some (s: option X) (v : term) : lambda v -> enc s == ext (@Some X) v -> exists s', s = Some s' /\ v = enc s'.
-  Proof.
-    intros lam_v H. unfold ext in H;cbn in H. unfold extT in H; cbn in H. redStep in H.
-    apply unique_normal_forms in H;[|Lproc..]. destruct s;simpl in H.
-    -injection H;eauto.
-    -discriminate H.
-  Qed.
-       
+  Definition option_enc : forall X : Type, registered X -> encodable (option X) := 
+  fun (X : Type) (intX : registered X) =>
+    fix encode (x : option X) : term :=
+    match x with
+    | Some x0 => lam (lam (var 1 (lam 0) (enc x0)))
+    | None => lam (lam (var 0 (lam 0)))
+    end.
 
+  Instance registered_option_enc X `{intX:registered X}: registered (@option X).
+  Proof.
+    eexists (option_enc intX).
+    -intros [];cbn. all:Lproc.
+    -intros [] [] [=]. now apply inj_enc in H0. easy.
+  Defined.
+
+  Lemma option_enc_correct X `{R__X:registered X} (H : option X) (H0 : term) :
+      proc H0 -> forall H1 : term, proc H1 -> ((enc H) H0) H1 >(<=2) match H with
+                                                             | Some x => H0 (lam 0) (enc x)
+                                                             | None => H1 (lam 0)
+                                                             end.
+  Proof.
+    intros. extract match.
+  Qed.
+
+Hint Resolve option_enc_correct : Lrewrite.
+
+(* now we must register the non-constant constructors*)
+
+Global Instance term_Some : computableTime' (@Some) (fun X R__X _ _ => (1,tt)).
+Proof.
+    extract constructor. solverec. 
+Defined.
+
+Global Instance term_None : computableTime' (@None) (fun X R__X => tt).
+Proof.
+    extract constructor. solverec. 
+Defined.
+
+(*
+Lemma oenc_correct_some X `{R__X:registered X} (s: option X) (v : term) : lambda v -> enc s == ext (@Some X) v -> exists s', s = Some s' /\ v = enc s'.
+Proof.
+  intros lam_v H. unfold ext in H;cbn in H. unfold extT in H; cbn in H. redStep in H.
+  apply unique_normal_forms in H;[|Lproc..]. destruct s;simpl in H.
+  -injection H;eauto.
+  -discriminate H.
+Qed.
+       
+*)
 
    (*
    Lemma none_equiv_some v : proc v -> ~ none == some v.
@@ -36,7 +69,6 @@ Section Fix_X.
      eapply eq_lam in H. inv H. symmetry. unfold some. clear H. old_Lsimpl.
    Qed.
     *)
-End Fix_X.
 
 Hint Resolve option_enc_correct : Lrewrite.
 
@@ -70,7 +102,8 @@ Section int.
                                                                                             Some a, Some b => callTime2 eqbT a b + 10
                                                                                           | _,_ => 8 end,tt)))). cbn.
   Proof.
-    extract. solverec.
+    extract. Unshelve.
+    8:{ solverec.
   Defined.
 
 End int.
